mechanization/theories/Core/Semantic/PER/Lemmas.v
@@ -834,6 +834,162 @@ Ltac invert_per_sort_elems := match_by_head per_sort_elem ltac:(fun H => directe
 (*   lia. *)
 (* Qed. *)
 
+Add Parametric Morphism {P : PtsSig} {pred_P : PredicativeSig P} : (per_typ pred_P)
+  with signature (@relation_equivalence (domain P)) ==> eq ==> eq ==> iff as per_typ_morphism_iff.
+Proof with mautosolve.
+  intros R R' HRR'.  
+  split; intro Horig; [gen R' | gen R];
+    induction Horig; econstructor;
+    apply_relation_equivalence; try reflexivity; try eassumption.
+Qed.
+
+Add Parametric Morphism {P : PtsSig} {pred_P : PredicativeSig P} : (per_typ pred_P)
+  with signature (@relation_equivalence (domain P)) ==> (@relation_equivalence (domain P)) as per_typ_morphism_relation_equivalence.
+Proof.
+  intros * H ? ?.
+  simpl.
+  rewrite H.
+  reflexivity.
+Qed.
+
+Lemma per_typ_right_irrel {P : PtsSig} {pred_P : PredicativeSig P} : forall a b b' R R',
+    {{ DF a ≈ b ∈ per_typ pred_P ↘ R }} ->
+    {{ DF a ≈ b' ∈ per_typ pred_P ↘ R' }} ->
+    R <~> R'.
+Proof.
+  intros * Horig.
+  induction Horig;
+    intros Hright; dependent destruction Hright.
+  - apply_relation_equivalence.
+    reflexivity.
+  - basic_invert_per_sort_elem H0.
+    apply_relation_equivalence.
+    reflexivity.
+  - basic_invert_per_sort_elem H.
+    apply_relation_equivalence.
+    reflexivity.
+  - eapply per_sort_elem_right_irrel; mauto.
+Qed.
+
+
+Lemma per_typ_sym {P} {pred_P : PredicativeSig P} : forall {R a b},
+    {{ DF a ≈ b ∈ per_typ pred_P ↘ R }} ->
+    {{ DF b ≈ a ∈ per_typ pred_P ↘ R }} /\
+      (forall m m',
+          {{ Dom m ≈ m' ∈ R }} ->
+          {{ Dom m' ≈ m ∈ R }}).
+Proof with mautosolve.
+  simpl.
+  induction 1; split.
+  - econstructor; mauto.
+  - apply_relation_equivalence.
+    intros.
+    eapply per_sort_sym'; mauto.
+  - assert (per_sort_elem pred_P s R b a) by (eapply per_sort_sym; mauto).
+    econstructor; mauto.
+  - intros.
+    eapply per_elem_sym; mauto.
+Qed.
+
+Corollary per_typ_left_irrel {P} {pred_P : PredicativeSig P} : forall R a b R' a',
+    {{ DF a ≈ b ∈ per_typ pred_P ↘ R }} ->
+    {{ DF a' ≈ b ∈ per_typ pred_P ↘ R' }} ->
+    R <~> R'.
+Proof.
+  intros * ?%per_typ_sym ?%per_typ_sym.
+  destruct_conjs.
+  eauto using per_typ_right_irrel.
+Qed.
+
+Corollary per_typ_cross_irrel {P} {pred_P : PredicativeSig P} : forall R a b R' b',
+    {{ DF a ≈ b ∈ per_typ pred_P ↘ R }} ->
+    {{ DF b' ≈ a ∈ per_typ pred_P ↘ R' }} ->
+    R <~> R'.
+Proof.
+  intros * ? ?%per_typ_sym.
+  destruct_conjs.
+  eauto using per_typ_right_irrel.
+Qed.
+
+Ltac do_per_typ_irrel_assert1 :=
+  let tactic_error o1 o2 := fail 2 "per_typ_irrel biconditional between" o1 "and" o2 "cannot be solved" in
+  match goal with
+  | H1 : {{ DF ^?a ≈ ^_ ∈ per_typ ?pred_P ↘ ?R1 }},
+      H2 : {{ DF ^?a ≈ ^_ ∈ per_typ ?pred_P ↘ ?R2 }} |- _ =>
+      assert_fails (unify R1 R2);
+      match goal with
+      | H : R1 <~> R2 |- _ => fail 1
+      | H : R2 <~> R1 |- _ => fail 1
+      | _ => assert (R1 <~> R2) by (eapply per_typ_right_irrel; [apply H1 | apply H2]) || tactic_error R1 R2
+      end
+  | H1 : {{ DF ^_ ≈ ^?b ∈ per_typ ?pred_P ↘ ?R1 }},
+      H2 : {{ DF ^_ ≈ ^?b ∈ per_typ ?pred_P ↘ ?R2 }} |- _ =>
+      assert_fails (unify R1 R2);
+      match goal with
+      | H : R1 <~> R2 |- _ => fail 1
+      | H : R2 <~> R1 |- _ => fail 1
+      | _ => assert (R1 <~> R2) by (eapply per_typ_left_irrel; [apply H1 | apply H2]) || tactic_error R1 R2
+      end
+  | H1 : {{ DF ^?a ≈ ^_ ∈ per_typ ?pred_P ↘ ?R1 }},
+      H2 : {{ DF ^_ ≈ ^?a ∈ per_typ ?pred_P ↘ ?R2 }} |- _ =>
+      (** Order matters less here as H1 and H2 cannot be exchanged *)
+      assert_fails (unify R1 R2);
+      match goal with
+      | H : R1 <~> R2 |- _ => fail 1
+      | H : R2 <~> R1 |- _ => fail 1
+      | _ => assert (R1 <~> R2) by (eapply per_typ_cross_irrel; [apply H1 | apply H2]) || tactic_error R1 R2
+      end
+  end.
+
+Ltac do_per_typ_irrel_assert :=
+  repeat do_per_typ_irrel_assert1.
+
+Ltac handle_per_typ_irrel :=
+  functional_eval_rewrite_clear;
+  do_per_typ_irrel_assert;
+  apply_relation_equivalence;
+  clear_dups.
+
+
+Lemma per_typ_trans {P} {pred_P : PredicativeSig P} : forall R a1 a2,
+    {{ DF a1 ≈ a2 ∈ per_typ pred_P ↘ R }} ->
+    (forall a3,
+        {{ DF a2 ≈ a3 ∈ per_typ pred_P ↘ R }} ->
+        {{ DF a1 ≈ a3 ∈ per_typ pred_P ↘ R }}) /\
+      (forall m1 m2 m3,
+          R m1 m2 ->
+          R m2 m3 ->
+          R m1 m3).
+Proof with mautosolve.
+  simpl.
+  induction 1.
+  - split.
+    + intros.
+      mauto.
+    + apply_relation_equivalence.      
+      eapply per_sort_trans'; mauto.
+  - split.
+    + intros.
+      dependent destruction H0.
+      * apply_relation_equivalence.
+        econstructor; mauto.
+      * assert (per_sort_elem pred_P s R a b) by (eapply per_sort_trans; mauto).
+        econstructor; mauto.
+    + apply_relation_equivalence.
+      eapply per_sort_elem_trans; mauto.
+Qed.
+
+#[export]
+Instance per_typ_PER {P} {pred_P : PredicativeSig P} {R} : PER (per_typ pred_P R).
+Proof.
+  split.
+  - intros x y H.
+    eapply (per_typ_sym H).
+  - intros x y z Hxy Hyz.
+    eapply (proj1 (per_typ_trans R x y Hxy) z Hyz).
+Qed.
+
+
 Add Parametric Morphism {P : PtsSig} {pred_P : PredicativeSig P} : (per_ctx_env pred_P)
     with signature (@relation_equivalence (env P)) ==> eq ==> eq ==> iff as per_ctx_env_morphism_iff.
 Proof with mautosolve.
